# triplets-pythagoriciens
### Round

Renvoie:

0^2 + 0^2 = 0^2
0^2 + 1^2 = 1^2
0^2 + 2^2 = 2^2
0^2 + 3^2 = 3^2
0^2 + 4^2 = 4^2
0^2 + 5^2 = 5^2
0^2 + 6^2 = 6^2
0^2 + 7^2 = 7^2
0^2 + 8^2 = 8^2
0^2 + 9^2 = 9^2
0^2 + 10^2 = 10^2
0^2 + 11^2 = 11^2
0^2 + 12^2 = 12^2
0^2 + 13^2 = 13^2
0^2 + 14^2 = 14^2
0^2 + 15^2 = 15^2
0^2 + 16^2 = 16^2
0^2 + 17^2 = 17^2
0^2 + 18^2 = 18^2
0^2 + 19^2 = 19^2
0^2 + 20^2 = 20^2
0^2 + 21^2 = 21^2
0^2 + 22^2 = 22^2
0^2 + 23^2 = 23^2
0^2 + 24^2 = 24^2
0^2 + 25^2 = 25^2
0^2 + 26^2 = 26^2
0^2 + 27^2 = 27^2
0^2 + 28^2 = 28^2
0^2 + 29^2 = 29^2
0^2 + 30^2 = 30^2
0^2 + 31^2 = 31^2
0^2 + 32^2 = 32^2
0^2 + 33^2 = 33^2
0^2 + 34^2 = 34^2
0^2 + 35^2 = 35^2
0^2 + 36^2 = 36^2
0^2 + 37^2 = 37^2
0^2 + 38^2 = 38^2
0^2 + 39^2 = 39^2
0^2 + 40^2 = 40^2
0^2 + 41^2 = 41^2
0^2 + 42^2 = 42^2
0^2 + 43^2 = 43^2
0^2 + 44^2 = 44^2
0^2 + 45^2 = 45^2
0^2 + 46^2 = 46^2
0^2 + 47^2 = 47^2
0^2 + 48^2 = 48^2
0^2 + 49^2 = 49^2
0^2 + 50^2 = 50^2
0^2 + 51^2 = 51^2
0^2 + 52^2 = 52^2
0^2 + 53^2 = 53^2
0^2 + 54^2 = 54^2
0^2 + 55^2 = 55^2
0^2 + 56^2 = 56^2
0^2 + 57^2 = 57^2
0^2 + 58^2 = 58^2
0^2 + 59^2 = 59^2
0^2 + 60^2 = 60^2
0^2 + 61^2 = 61^2
0^2 + 62^2 = 62^2
0^2 + 63^2 = 63^2
0^2 + 64^2 = 64^2
0^2 + 65^2 = 65^2
0^2 + 66^2 = 66^2
0^2 + 67^2 = 67^2
0^2 + 68^2 = 68^2
0^2 + 69^2 = 69^2
0^2 + 70^2 = 70^2
0^2 + 71^2 = 71^2
0^2 + 72^2 = 72^2
0^2 + 73^2 = 73^2
0^2 + 74^2 = 74^2
0^2 + 75^2 = 75^2
0^2 + 76^2 = 76^2
0^2 + 77^2 = 77^2
0^2 + 78^2 = 78^2
0^2 + 79^2 = 79^2
0^2 + 80^2 = 80^2
0^2 + 81^2 = 81^2
0^2 + 82^2 = 82^2
0^2 + 83^2 = 83^2
0^2 + 84^2 = 84^2
0^2 + 85^2 = 85^2
0^2 + 86^2 = 86^2
0^2 + 87^2 = 87^2
0^2 + 88^2 = 88^2
0^2 + 89^2 = 89^2
0^2 + 90^2 = 90^2
0^2 + 91^2 = 91^2
0^2 + 92^2 = 92^2
0^2 + 93^2 = 93^2
0^2 + 94^2 = 94^2
0^2 + 95^2 = 95^2
0^2 + 96^2 = 96^2
0^2 + 97^2 = 97^2
0^2 + 98^2 = 98^2
0^2 + 99^2 = 99^2
0^2 + 100^2 = 100^2
1^2 + 0^2 = 1^2
2^2 + 0^2 = 2^2
3^2 + 0^2 = 3^2
3^2 + 4^2 = 5^2
4^2 + 0^2 = 4^2
4^2 + 3^2 = 5^2
5^2 + 0^2 = 5^2
5^2 + 12^2 = 13^2
6^2 + 0^2 = 6^2
6^2 + 8^2 = 10^2
7^2 + 0^2 = 7^2
7^2 + 24^2 = 25^2
8^2 + 0^2 = 8^2
8^2 + 6^2 = 10^2
8^2 + 15^2 = 17^2
9^2 + 0^2 = 9^2
9^2 + 12^2 = 15^2
9^2 + 40^2 = 41^2
10^2 + 0^2 = 10^2
10^2 + 24^2 = 26^2
11^2 + 0^2 = 11^2
11^2 + 60^2 = 61^2
12^2 + 0^2 = 12^2
12^2 + 5^2 = 13^2
12^2 + 9^2 = 15^2
12^2 + 16^2 = 20^2
12^2 + 35^2 = 37^2
13^2 + 0^2 = 13^2
13^2 + 84^2 = 85^2
14^2 + 0^2 = 14^2
14^2 + 48^2 = 50^2
15^2 + 0^2 = 15^2
15^2 + 8^2 = 17^2
15^2 + 20^2 = 25^2
15^2 + 36^2 = 39^2
16^2 + 0^2 = 16^2
16^2 + 12^2 = 20^2
16^2 + 30^2 = 34^2
16^2 + 63^2 = 65^2
17^2 + 0^2 = 17^2
18^2 + 0^2 = 18^2
18^2 + 24^2 = 30^2
18^2 + 80^2 = 82^2
19^2 + 0^2 = 19^2
20^2 + 0^2 = 20^2
20^2 + 15^2 = 25^2
20^2 + 21^2 = 29^2
20^2 + 48^2 = 52^2
21^2 + 0^2 = 21^2
21^2 + 20^2 = 29^2
21^2 + 28^2 = 35^2
21^2 + 72^2 = 75^2
22^2 + 0^2 = 22^2
23^2 + 0^2 = 23^2
24^2 + 0^2 = 24^2
24^2 + 7^2 = 25^2
24^2 + 10^2 = 26^2
24^2 + 18^2 = 30^2
24^2 + 32^2 = 40^2
24^2 + 45^2 = 51^2
24^2 + 70^2 = 74^2
25^2 + 0^2 = 25^2
25^2 + 60^2 = 65^2
26^2 + 0^2 = 26^2
27^2 + 0^2 = 27^2
27^2 + 36^2 = 45^2
28^2 + 0^2 = 28^2
28^2 + 21^2 = 35^2
28^2 + 45^2 = 53^2
28^2 + 96^2 = 100^2
29^2 + 0^2 = 29^2
30^2 + 0^2 = 30^2
30^2 + 16^2 = 34^2
30^2 + 40^2 = 50^2
30^2 + 72^2 = 78^2
31^2 + 0^2 = 31^2
32^2 + 0^2 = 32^2
32^2 + 24^2 = 40^2
32^2 + 60^2 = 68^2
33^2 + 0^2 = 33^2
33^2 + 44^2 = 55^2
33^2 + 56^2 = 65^2
34^2 + 0^2 = 34^2
35^2 + 0^2 = 35^2
35^2 + 12^2 = 37^2
35^2 + 84^2 = 91^2
36^2 + 0^2 = 36^2
36^2 + 15^2 = 39^2
36^2 + 27^2 = 45^2
36^2 + 48^2 = 60^2
36^2 + 77^2 = 85^2
37^2 + 0^2 = 37^2
38^2 + 0^2 = 38^2
39^2 + 0^2 = 39^2
39^2 + 52^2 = 65^2
39^2 + 80^2 = 89^2
40^2 + 0^2 = 40^2
40^2 + 9^2 = 41^2
40^2 + 30^2 = 50^2
40^2 + 42^2 = 58^2
40^2 + 75^2 = 85^2
41^2 + 0^2 = 41^2
42^2 + 0^2 = 42^2
42^2 + 40^2 = 58^2
42^2 + 56^2 = 70^2
43^2 + 0^2 = 43^2
44^2 + 0^2 = 44^2
44^2 + 33^2 = 55^2
45^2 + 0^2 = 45^2
45^2 + 24^2 = 51^2
45^2 + 28^2 = 53^2
45^2 + 60^2 = 75^2
46^2 + 0^2 = 46^2
47^2 + 0^2 = 47^2
48^2 + 0^2 = 48^2
48^2 + 14^2 = 50^2
48^2 + 20^2 = 52^2
48^2 + 36^2 = 60^2
48^2 + 55^2 = 73^2
48^2 + 64^2 = 80^2
49^2 + 0^2 = 49^2
50^2 + 0^2 = 50^2
51^2 + 0^2 = 51^2
51^2 + 68^2 = 85^2
52^2 + 0^2 = 52^2
52^2 + 39^2 = 65^2
53^2 + 0^2 = 53^2
54^2 + 0^2 = 54^2
54^2 + 72^2 = 90^2
55^2 + 0^2 = 55^2
55^2 + 48^2 = 73^2
56^2 + 0^2 = 56^2
56^2 + 33^2 = 65^2
56^2 + 42^2 = 70^2
57^2 + 0^2 = 57^2
57^2 + 76^2 = 95^2
58^2 + 0^2 = 58^2
59^2 + 0^2 = 59^2
60^2 + 0^2 = 60^2
60^2 + 11^2 = 61^2
60^2 + 25^2 = 65^2
60^2 + 32^2 = 68^2
60^2 + 45^2 = 75^2
60^2 + 63^2 = 87^2
60^2 + 80^2 = 100^2
61^2 + 0^2 = 61^2
62^2 + 0^2 = 62^2
63^2 + 0^2 = 63^2
63^2 + 16^2 = 65^2
63^2 + 60^2 = 87^2
64^2 + 0^2 = 64^2
64^2 + 48^2 = 80^2
65^2 + 0^2 = 65^2
65^2 + 72^2 = 97^2
66^2 + 0^2 = 66^2
67^2 + 0^2 = 67^2
68^2 + 0^2 = 68^2
68^2 + 51^2 = 85^2
69^2 + 0^2 = 69^2
70^2 + 0^2 = 70^2
70^2 + 24^2 = 74^2
71^2 + 0^2 = 71^2
72^2 + 0^2 = 72^2
72^2 + 21^2 = 75^2
72^2 + 30^2 = 78^2
72^2 + 54^2 = 90^2
72^2 + 65^2 = 97^2
73^2 + 0^2 = 73^2
74^2 + 0^2 = 74^2
75^2 + 0^2 = 75^2
75^2 + 40^2 = 85^2
76^2 + 0^2 = 76^2
76^2 + 57^2 = 95^2
77^2 + 0^2 = 77^2
77^2 + 36^2 = 85^2
78^2 + 0^2 = 78^2
79^2 + 0^2 = 79^2
80^2 + 0^2 = 80^2
80^2 + 18^2 = 82^2
80^2 + 39^2 = 89^2
80^2 + 60^2 = 100^2
81^2 + 0^2 = 81^2
82^2 + 0^2 = 82^2
83^2 + 0^2 = 83^2
84^2 + 0^2 = 84^2
84^2 + 13^2 = 85^2
84^2 + 35^2 = 91^2
85^2 + 0^2 = 85^2
86^2 + 0^2 = 86^2
87^2 + 0^2 = 87^2
88^2 + 0^2 = 88^2
89^2 + 0^2 = 89^2
90^2 + 0^2 = 90^2
91^2 + 0^2 = 91^2
92^2 + 0^2 = 92^2
93^2 + 0^2 = 93^2
94^2 + 0^2 = 94^2
95^2 + 0^2 = 95^2
96^2 + 0^2 = 96^2
96^2 + 28^2 = 100^2
97^2 + 0^2 = 97^2
98^2 + 0^2 = 98^2
99^2 + 0^2 = 99^2
100^2 + 0^2 = 100^2
NIL

## License

Specify license here

